theories/interop/linking_wp.v
@@ -7,115 +7,45 @@ From iris.proofmode Require Import proofmode.
 
 (* FIXME: the proofs in this file need cleanup *)
 
-Class state_interp_for_linking
-      {val pubstate : Type} {Σ : gFunctors}
-      (public_state_interp : pubstate → iProp Σ)
-      (Λ : mlanguage val pubstate) (state_interp : state Λ → iProp Σ)
-:= StateInterpForLinking {
-  private_state_interp : Λ.(private_state) → iProp Σ;
-
-  state_interp_split σ pubσ privσ :
-    split_state σ pubσ privσ →
-    state_interp σ ==∗ public_state_interp pubσ ∗ private_state_interp privσ;
-
-  state_interp_join σ pubσ privσ :
-    split_state σ pubσ privσ →
-    public_state_interp pubσ ∗ private_state_interp privσ ==∗ state_interp σ
-}.
-
 Section Linking_logic.
 Context {hlc : has_lc}.
 Context {Σ : gFunctors}.
 Context {val pubstate : Type}.
 Context (Λ1 Λ2 : mlanguage val pubstate).
-
-Context (public_state_interp : pubstate → iProp Σ).
-Context (state_interp1 : state Λ1 → iProp Σ).
-Context (state_interp2 : state Λ2 → iProp Σ).
-Context (SIL1 : state_interp_for_linking public_state_interp Λ1 state_interp1).
-Context (SIL2 : state_interp_for_linking public_state_interp Λ2 state_interp2).
+Context `{!publicStateInterp pubstate Σ}.
+Context `{!mlangGS hlc val pubstate Σ Λ1}.
+Context `{!mlangGS hlc val pubstate Σ Λ2}.
 
 Implicit Types P : iProp Σ.
 Implicit Types Φ : val → iProp Σ.
 Implicit Types v : val.
 Implicit Types T : string -d> list val -d> (val -d> iPropO Σ) -d> iPropO Σ.
 
-Definition valid_split (Λ : mlanguage val pubstate)
-                       (pubσ : pubstate) (privσ : Λ.(private_state)) : Prop :=
-  ∃ σ, Λ.(split_state) σ pubσ privσ.
-
-Class can_link_lang := CanLinkLangs {
-  lang1_state_rel : Λ1.(state) → Λ1.(state) → Prop;
-  lang2_state_rel : Λ2.(state) → Λ2.(state) → Prop;
-  lang1_state_rel_refl :> Reflexive lang1_state_rel;
-  lang2_state_rel_refl :> Reflexive lang2_state_rel;
-  lang1_state_rel_trans :> Transitive lang1_state_rel;
-  lang2_state_rel_trans :> Transitive lang2_state_rel;
-
-  lang1_state_rel_step p e σ X :
-    Λ1.(head_step) p (e, σ) X →
-    Λ1.(head_step) p (e, σ) (λ '(e', σ'), X (e', σ') ∧ lang1_state_rel σ σ');
-  lang2_state_rel_step p e σ X :
-    Λ2.(head_step) p (e, σ) X →
-    Λ2.(head_step) p (e, σ) (λ '(e', σ'), X (e', σ') ∧ lang2_state_rel σ σ');
-
-  lang1_state_rel_valid_split σ1 pubσ privσ1 σ1' pubσ' privσ1' privσ2 :
-    Λ1.(split_state) σ1 pubσ privσ1 →
-    valid_split Λ2 pubσ privσ2 →
-    lang1_state_rel σ1 σ1' →
-    Λ1.(split_state) σ1' pubσ' privσ1' →
-    valid_split Λ2 pubσ' privσ2;
-  lang2_state_rel_valid_split σ2 pubσ privσ2 σ2' pubσ' privσ2' privσ1 :
-    Λ2.(split_state) σ2 pubσ privσ2 →
-    valid_split Λ1 pubσ privσ1 →
-    lang2_state_rel σ2 σ2' →
-    Λ2.(split_state) σ2' pubσ' privσ2' →
-    valid_split Λ1 pubσ' privσ1;
-}.
-
-Lemma lang1_state_rel_prim_step `{can_link_lang} p e σ X :
-  prim_step p (e, σ) X →
-  prim_step p (e, σ) (λ '(e', σ'), X (e', σ') ∧ lang1_state_rel σ σ').
-Proof using.
-  intros (K & e' & -> & Hstep%lang1_state_rel_step). eexists; eauto.
-Qed.
-Lemma lang2_state_rel_prim_step `{can_link_lang} p e σ X :
-  prim_step p (e, σ) X →
-  prim_step p (e, σ) (λ '(e', σ'), X (e', σ') ∧ lang2_state_rel σ σ').
-Proof using.
-  intros (K & e' & -> & Hstep%lang2_state_rel_step). eexists; eauto.
-Qed.
-
-Context `{can_link_lang}.
-
 Definition link_state_interp (st : (link_lang Λ1 Λ2).(state)) : iProp Σ :=
   match st with
   | LinkSt pubσ privσ1 privσ2 =>
       public_state_interp pubσ ∗
       private_state_interp privσ1 ∗
-      private_state_interp privσ2 ∗
-      ⌜valid_split Λ1 pubσ privσ1 ∧ valid_split Λ2 pubσ privσ2⌝
+      private_state_interp privσ2
   | LinkSt1 σ1 privσ2 =>
-      state_interp1 σ1 ∗ private_state_interp privσ2 ∗
-      ⌜∃ σ1_0 pubσ0 privσ1_0,
-          lang1_state_rel σ1_0 σ1 ∧
-          Λ1.(split_state) σ1_0 pubσ0 privσ1_0 ∧
-          valid_split Λ2 pubσ0 privσ2⌝
-
+      state_interp σ1 ∗ private_state_interp privσ2
   | LinkSt2 privσ1 σ2 =>
-      private_state_interp privσ1 ∗ state_interp2 σ2 ∗
-      ⌜∃ σ2_0 pubσ0 privσ2_0,
-          lang2_state_rel σ2_0 σ2 ∧
-          Λ2.(split_state) σ2_0 pubσ0 privσ2_0 ∧
-          valid_split Λ1 pubσ0 privσ1⌝
+      private_state_interp privσ1 ∗ state_interp σ2
   end.
 
-Instance link_melocotonGS {INVG: invGS_gen hlc Σ} :
-  melocotonGS_gen hlc val pubstate (link_lang Λ1 Λ2) Σ
-:= {
-  iris_invGS := INVG;
+Program Instance link_mlangGS : mlangGS hlc val pubstate Σ (link_lang Λ1 Λ2) := {
   state_interp := link_state_interp;
+  private_state_interp := (λ '(privσ1, privσ2),
+    private_state_interp privσ1 ∗ private_state_interp privσ2)%I;
 }.
+Next Obligation.
+  simpl. iIntros (σ pubσ privσ). inversion 1; subst.
+  iIntros "(? & ? & ?)". by iFrame.
+Qed.
+Next Obligation.
+  simpl. iIntros (σ pubσ privσ). inversion 1; subst.
+  iIntros "(? & ? & ?)". by iFrame.
+Qed.
 
 Lemma proj1_prog_union (pe1: mlanguage.prog Λ1) (pe2: mlanguage.prog Λ2) :
   dom pe1 ## dom pe2 →
@@ -143,10 +73,10 @@ Proof using.
   { rewrite lookup_omap /= lookup_fmap. by destruct (pe1 !! fname). }
 Qed.
 
-Definition link_environ (INVG: invGS_gen hlc Σ)
-  (pe1 : @prog_environ hlc _ _ Λ1 Σ (IrisG INVG state_interp1))
-  (pe2 : @prog_environ hlc _ _ Λ2 Σ (IrisG INVG state_interp2))
-: @prog_environ _ _ _ (link_lang Λ1 Λ2) Σ (IrisG INVG link_state_interp) :=
+Definition link_environ `{!invGS_gen hlc Σ}
+  (pe1 : @prog_environ _ _ _ _ _ _ Λ1 _)
+  (pe2 : @prog_environ _ _ _ _ _ _ Λ2 _)
+: @prog_environ _ _ _ _ _ _ (link_lang Λ1 Λ2) _ :=
 {|
   prog := fmap inl (prog pe1) ∪ fmap inr (prog pe2);
   T := λ fname vs Φ,
@@ -154,9 +84,9 @@ Definition link_environ (INVG: invGS_gen hlc Σ)
      (T pe1 fname vs Φ ∨ T pe2 fname vs Φ))%I;
 |}.
 
-Class can_link_prog (INVG: invGS_gen hlc Σ)
-  (pe1 : @prog_environ hlc _ _ Λ1 Σ (IrisG INVG state_interp1))
-  (pe2 : @prog_environ hlc _ _ Λ2 Σ (IrisG INVG state_interp2))
+Class can_link_prog `{!invGS_gen hlc Σ}
+  (pe1 : @prog_environ _ _ _ _ _ _ Λ1 _)
+  (pe2 : @prog_environ _ _ _ _ _ _ Λ2 _)
 := CanLinkProgs {
   can_link_disj :
     dom (prog pe1) ## dom (prog pe2);
@@ -170,18 +100,18 @@ Class can_link_prog (INVG: invGS_gen hlc Σ)
       ∃ e1, ⌜apply_func func vs = Some e1⌝ ∗ ▷ WP e1 @ pe1; E {{ Φ }};
 }.
 
-Lemma wp_link_call (INVG: invGS_gen hlc Σ)
-  (pe1 : @prog_environ hlc _ _ Λ1 Σ (IrisG INVG state_interp1))
-  (pe2 : @prog_environ hlc _ _ Λ2 Σ (IrisG INVG state_interp2))
+Lemma wp_link_call `{!invGS_gen hlc Σ}
+  (pe1 : @prog_environ _ _ _ _ _ _ Λ1 _)
+  (pe2 : @prog_environ _ _ _ _ _ _ Λ2 _)
   E k fn vs (Φ : val → iProp Σ) fname
 :
-  let pe := link_environ INVG pe1 pe2 in
+  let pe := link_environ pe1 pe2 in
   prog pe !! fname = Some fn →
   WP LkE (LinkRunFunction Λ1 Λ2 fn vs) k @ pe; E {{ Φ }} -∗
   WP LkE (LinkExprCall Λ1 Λ2 fname vs) k @ pe; E {{ Φ }}.
 Proof using.
   iIntros (pe Hfn) "Hwp".
-  iApply (@wp_unfold _ _ _ (link_lang Λ1 Λ2)). rewrite /wp_pre.
+  iApply (@wp_unfold _ _ _ _ _ _ (link_lang Λ1 Λ2)). rewrite /wp_pre.
   iIntros (σ) "[Hσ %Hmatch]". iModIntro. iRight; iRight.
   inversion Hmatch; subst.
   iSplitR.
@@ -192,13 +122,13 @@ Proof using.
   iModIntro. iNext. iModIntro. iExists _, _. iSplitR; first done. iFrame.
 Qed.
 
-Lemma wp_link_run_function_1 (INVG: invGS_gen hlc Σ)
-  (pe1 : @prog_environ hlc _ _ Λ1 Σ (IrisG INVG state_interp1))
-  (pe2 : @prog_environ hlc _ _ Λ2 Σ (IrisG INVG state_interp2))
+Lemma wp_link_run_function_1 `{!invGS_gen hlc Σ}
+  (pe1 : @prog_environ _ _ _ _ _ _ Λ1 _)
+  (pe2 : @prog_environ _ _ _ _ _ _ Λ2 _)
   E k2 k fn arg fname (Φ : val → iProp Σ) (Ξ : val → iProp Σ)
 :
-  let pe := link_environ INVG pe1 pe2 in
-  can_link_prog INVG pe1 pe2 →
+  let pe := link_environ pe1 pe2 in
+  can_link_prog pe1 pe2 →
   prog pe1 !! fname = Some fn →
   T pe2 fname arg Ξ -∗
   (∀ e1, ⌜apply_func fn arg = Some e1⌝ -∗
@@ -207,30 +137,29 @@ Lemma wp_link_run_function_1 (INVG: invGS_gen hlc Σ)
   WP LkE (LinkRunFunction Λ1 Λ2 (inl fn) arg) (inr k2 :: k) @ pe; E {{ Φ }}.
 Proof using.
   iIntros (pe Hcan_link Hfn) "HTΞ Hwp".
-  iApply (@wp_unfold _ _ _ (link_lang Λ1 Λ2)). rewrite /wp_pre.
+  iApply (@wp_unfold _ _ _ _ _ _ (link_lang Λ1 Λ2)). rewrite /wp_pre.
   iIntros (σ) "[Hσ %Hmatch]". inversion Hmatch; subst.
   iRight; iRight.
   iPoseProof (can_link_spec2 _ _ _ _ E Hfn with "HTΞ") as (? Happlyfunc) "Hwpcall".
 
-  iDestruct "Hσ" as "(Hpubσ & Hprivσ1 & Hprivσ2 & %Hvsplit1 & %Hvsplit2)".
+  iDestruct "Hσ" as "(Hpubσ & Hprivσ1 & Hprivσ2)".
   iModIntro. iSplitR.
-  { iPureIntro. destruct Hvsplit1 as (? & ?). exists (λ _, True). eexists _, (LkE _ []). split; [done|].
-    eapply RunFunction1S; eauto. }
+  { iPureIntro. exists (λ _, True). eexists _, (LkE _ []). split; [done|].
+    destruct (merge_split_state pubσ privσ1) as [? ?]. eapply RunFunction1S; eauto. }
   iIntros (X Hstep'). destruct Hstep' as (K' & [se1' k1'] & ? & Hstep'). simpl in *; simplify_eq.
   inversion Hstep'; simplify_eq/=; []. iModIntro. iNext.
   iMod (@state_interp_join _ _ _ _ Λ1 with "[$Hprivσ1 $Hpubσ]") as "Hσ1". eassumption.
-  iModIntro. iExists _, _. iSplitR; first done. iFrame "Hprivσ2 Hσ1". iSplitR.
-  { iPureIntro. do 3 eexists. repeat split; eauto. reflexivity. }
+  iModIntro. iExists _, _. iSplitR; first done. iFrame "Hprivσ2 Hσ1".
   by iApply "Hwp".
 Qed.
 
-Lemma wp_link_run_function_2 (INVG: invGS_gen hlc Σ)
-  (pe1 : @prog_environ hlc _ _ Λ1 Σ (IrisG INVG state_interp1))
-  (pe2 : @prog_environ hlc _ _ Λ2 Σ (IrisG INVG state_interp2))
+Lemma wp_link_run_function_2 `{!invGS_gen hlc Σ}
+  (pe1 : @prog_environ _ _ _ _ _ _ Λ1 _)
+  (pe2 : @prog_environ _ _ _ _ _ _ Λ2 _)
   E k1 k fn arg fname (Φ : val → iProp Σ) (Ξ : val → iProp Σ)
 :
-  let pe := link_environ INVG pe1 pe2 in
-  can_link_prog INVG pe1 pe2 →
+  let pe := link_environ pe1 pe2 in
+  can_link_prog pe1 pe2 →
   prog pe2 !! fname = Some fn →
   T pe1 fname arg Ξ -∗
   (∀ e2, ⌜apply_func fn arg = Some e2⌝ -∗
@@ -239,79 +168,76 @@ Lemma wp_link_run_function_2 (INVG: invGS_gen hlc Σ)
   WP LkE (LinkRunFunction Λ1 Λ2 (inr fn) arg) (inl k1 :: k) @ pe; E {{ Φ }}.
 Proof using.
   iIntros (pe Hcan_link Hfn) "HTΞ Hwp".
-  iApply (@wp_unfold _ _ _ (link_lang Λ1 Λ2)). rewrite /wp_pre.
+  iApply (@wp_unfold _ _ _ _ _ _ (link_lang Λ1 Λ2)). rewrite /wp_pre.
   iIntros (σ) "[Hσ %Hmatch]". inversion Hmatch; subst.
   iRight; iRight.
   iPoseProof (can_link_spec1 _ _ _ _ E Hfn with "HTΞ") as (? Happlyfunc) "Hwpcall".
 
-  iDestruct "Hσ" as "(Hpubσ & Hprivσ1 & Hprivσ2 & %Hvsplit1 & %Hvsplit2)".
+  iDestruct "Hσ" as "(Hpubσ & Hprivσ1 & Hprivσ2)".
   iModIntro. iSplitR.
-  { iPureIntro. destruct Hvsplit2 as (? & ?). exists (λ _, True). eexists _, (LkE _ []). split; [done|].
-    eapply RunFunction2S; eauto. }
+  { iPureIntro. exists (λ _, True). eexists _, (LkE _ []). split; [done|].
+    destruct (merge_split_state pubσ privσ2) as [? ?]. eapply RunFunction2S; eauto. }
   iIntros (X Hstep'). destruct Hstep' as (K' & [se2' k2'] & ? & Hstep'). simpl in *; simplify_eq.
   inversion Hstep'; simplify_eq/=; []. iModIntro. iNext.
   iMod (@state_interp_join _ _ _ _ Λ2 with "[$Hprivσ2 $Hpubσ]") as "Hσ2". eassumption.
-  iModIntro. iExists _, _. iSplitR; first done. iFrame "Hprivσ1 Hσ2". iSplitR.
-  { iPureIntro. do 3 eexists. repeat split; eauto. reflexivity. }
+  iModIntro. iExists _, _. iSplitR; first done. iFrame "Hprivσ1 Hσ2".
   by iApply "Hwp".
 Qed.
 
-Lemma wp_link_retval_1 (INVG: invGS_gen hlc Σ)
-  (pe1 : @prog_environ hlc _ _ Λ1 Σ (IrisG INVG state_interp1))
-  (pe2 : @prog_environ hlc _ _ Λ2 Σ (IrisG INVG state_interp2))
+Lemma wp_link_retval_1 `{!invGS_gen hlc Σ}
+  (pe1 : @prog_environ _ _ _ _ _ _ Λ1 _)
+  (pe2 : @prog_environ _ _ _ _ _ _ Λ2 _)
   E k1 v (Φ : val → iProp Σ)
 :
-  let pe := link_environ INVG pe1 pe2 in
+  let pe := link_environ pe1 pe2 in
   WP LkSE (LinkExpr1 Λ1 Λ2 (fill k1 (of_val Λ1 v))) @ pe; E {{ Φ }} -∗
   WP LkE (LinkExprV Λ1 Λ2 v) [inl k1] @ pe; E {{ Φ }}.
 Proof using.
   iIntros (pe) "Hwp".
-  iApply (@wp_unfold _ _ _ (link_lang Λ1 Λ2)). rewrite /wp_pre.
+  iApply (@wp_unfold _ _ _ _ _ _ (link_lang Λ1 Λ2)). rewrite /wp_pre.
   iIntros (σ) "[Hσ %Hmatch']". inversion Hmatch'; subst. iModIntro. iRight. iRight.
-  iDestruct "Hσ" as "(Hpub & Hpriv1 & Hpriv2 & %Hvsplit1 & %Hvsplit2)".
+  iDestruct "Hσ" as "(Hpub & Hpriv1 & Hpriv2)".
   iSplitR.
-  { iPureIntro. apply head_prim_reducible. destruct Hvsplit1 as [? ?].
-    exists (λ _, True). eapply Ret1S; eauto. }
+  { iPureIntro. apply head_prim_reducible. exists (λ _, True).
+    destruct (merge_split_state pubσ privσ1) as [? ?]. eapply Ret1S; eauto. }
   iIntros (X Hstep'). destruct Hstep' as (K' & [se1' k1'] & ? & Hstep'). simplify_eq/=.
   inversion Hstep'; simplify_eq/=; [].
   iModIntro. iNext.
   iMod (@state_interp_join _ _ _ _ Λ1 with "[$Hpriv1 $Hpub]") as "H1". eassumption.
-  iModIntro. iExists _, _. iSplitR; first done. iFrame "Hpriv2 H1". iSplitR.
-  { iPureIntro. do 3 eexists. repeat split; eauto. reflexivity. }
+  iModIntro. iExists _, _. iSplitR; first done. iFrame "Hpriv2 H1".
   by iFrame.
 Qed.
 
-Lemma wp_link_retval_2 (INVG: invGS_gen hlc Σ)
-  (pe1 : @prog_environ hlc _ _ Λ1 Σ (IrisG INVG state_interp1))
-  (pe2 : @prog_environ hlc _ _ Λ2 Σ (IrisG INVG state_interp2))
+Lemma wp_link_retval_2 `{!invGS_gen hlc Σ}
+  (pe1 : @prog_environ _ _ _ _ _ _ Λ1 _)
+  (pe2 : @prog_environ _ _ _ _ _ _ Λ2 _)
   E k2 v (Φ : val → iProp Σ)
 :
-  let pe := link_environ INVG pe1 pe2 in
+  let pe := link_environ pe1 pe2 in
   WP LkSE (LinkExpr2 Λ1 Λ2 (fill k2 (of_val Λ2 v))) @ pe; E {{ Φ }} -∗
   WP LkE (LinkExprV Λ1 Λ2 v) [inr k2] @ pe; E {{ Φ }}.
 Proof using.
   iIntros (pe) "Hwp".
-  iApply (@wp_unfold _ _ _ (link_lang Λ1 Λ2)). rewrite /wp_pre.
+  iApply (@wp_unfold _ _ _ _ _ _ (link_lang Λ1 Λ2)). rewrite /wp_pre.
   iIntros (σ) "[Hσ %Hmatch']". inversion Hmatch'; subst. iModIntro. iRight. iRight.
-  iDestruct "Hσ" as "(Hpub & Hpriv1 & Hpriv2 & %Hvsplit1 & %Hvsplit2)".
+  iDestruct "Hσ" as "(Hpub & Hpriv1 & Hpriv2)".
   iSplitR.
-  { iPureIntro. apply head_prim_reducible. destruct Hvsplit2 as [? ?].
-    eexists (λ _, True). eapply Ret2S; eauto. }
+  { iPureIntro. apply head_prim_reducible. eexists (λ _, True).
+    destruct (merge_split_state pubσ privσ2). eapply Ret2S; eauto. }
   iIntros (X Hstep'). destruct Hstep' as (K' & [se2' k2'] & ? & Hstep'). simplify_eq/=.
   inversion Hstep'; simplify_eq/=; [].
   iModIntro. iNext.
   iMod (@state_interp_join _ _ _ _ Λ2 with "[$Hpriv2 $Hpub]") as "H2". eassumption.
-  iModIntro. iExists _, _. iSplitR; first done. iFrame "Hpriv1 H2". iSplitR.
-  { iPureIntro. do 3 eexists. repeat split; eauto. reflexivity. }
+  iModIntro. iExists _, _. iSplitR; first done. iFrame "Hpriv1 H2".
   by iFrame.
 Qed.
 
-Lemma wp_link_extcall_1 (INVG: invGS_gen hlc Σ)
-  (pe1 : @prog_environ hlc _ _ Λ1 Σ (IrisG INVG state_interp1))
-  (pe2 : @prog_environ hlc _ _ Λ2 Σ (IrisG INVG state_interp2))
+Lemma wp_link_extcall_1 `{!invGS_gen hlc Σ}
+  (pe1 : @prog_environ _ _ _ _ _ _ Λ1 _)
+  (pe2 : @prog_environ _ _ _ _ _ _ Λ2 _)
   E k1 fn_name arg (Φ : val → iProp Σ) (Ξ : val → iProp Σ)
 :
-  let pe := link_environ INVG pe1 pe2 in
+  let pe := link_environ pe1 pe2 in
   prog pe1 !! fn_name = None →
   prog pe2 !! fn_name = None →
   T pe1 fn_name arg Ξ -∗
@@ -323,7 +249,7 @@ Proof using.
   iIntros (pe Hfn1 Hfn2) "HTΞ HΞ Hwp".
   assert (Hpef: prog pe !! fn_name = None).
   { apply lookup_union_None. rewrite !lookup_fmap Hfn1 Hfn2 //. }
-  iApply (@wp_unfold _ _ _ (link_lang Λ1 Λ2)). rewrite /wp_pre.
+  iApply (@wp_unfold _ _ _ _ _ _ (link_lang Λ1 Λ2)). rewrite /wp_pre.
   iIntros (σ) "[Hσ %Hmatch']". inversion Hmatch'; subst.
   iModIntro. iRight; iLeft. iExists _, _, [inl k1]. iSplitR; [by eauto|].
   iSplitR; first by eauto. iModIntro. iFrame "Hσ". iExists Ξ. iSplitL "HTΞ".
@@ -332,12 +258,12 @@ Proof using.
   by iApply "Hwp".
 Qed.
 
-Lemma wp_link_extcall_2 (INVG: invGS_gen hlc Σ)
-  (pe1 : @prog_environ hlc _ _ Λ1 Σ (IrisG INVG state_interp1))
-  (pe2 : @prog_environ hlc _ _ Λ2 Σ (IrisG INVG state_interp2))
+Lemma wp_link_extcall_2 `{!invGS_gen hlc Σ}
+  (pe1 : @prog_environ _ _ _ _ _ _ Λ1 _)
+  (pe2 : @prog_environ _ _ _ _ _ _ Λ2 _)
   E k2 fn_name arg (Φ : val → iProp Σ) (Ξ : val → iProp Σ)
 :
-  let pe := link_environ INVG pe1 pe2 in
+  let pe := link_environ pe1 pe2 in
   prog pe1 !! fn_name = None →
   prog pe2 !! fn_name = None →
   T pe2 fn_name arg Ξ -∗
@@ -349,7 +275,7 @@ Proof using.
   iIntros (pe Hfn1 Hfn2) "HTΞ HΞ Hwp".
   assert (Hpef: prog pe !! fn_name = None).
   { apply lookup_union_None. rewrite !lookup_fmap Hfn1 Hfn2 //. }
-  iApply (@wp_unfold _ _ _ (link_lang Λ1 Λ2)). rewrite /wp_pre.
+  iApply (@wp_unfold _ _ _ _ _ _ (link_lang Λ1 Λ2)). rewrite /wp_pre.
   iIntros (σ) "[Hσ %Hmatch']". inversion Hmatch'; subst.
   iModIntro. iRight; iLeft. iExists _, _, [inr k2]. iSplitR; [by eauto|].
   iSplitR; first by eauto.
@@ -359,9 +285,9 @@ Proof using.
   by iApply "Hwp".
 Qed.
 
-Lemma link_head_step_call_ext_1_inv INVG pe1 pe2 K f vs σ1 privσ2 X :
-  let pe := link_environ INVG pe1 pe2 in
-  can_link_prog INVG pe1 pe2 →
+Lemma link_head_step_call_ext_1_inv `{!invGS_gen hlc Σ} pe1 pe2 K f vs σ1 privσ2 X :
+  let pe := link_environ pe1 pe2 in
+  can_link_prog pe1 pe2 →
   prog pe1 !! f = None →
   head_step (prog pe) (LkSE (LinkExpr1 Λ1 Λ2 (fill K (of_class Λ1 (ExprCall f vs)))),
                        LinkSt1 σ1 privσ2) X →
@@ -376,7 +302,7 @@ Proof using.
     rewrite proj1_prog_union in HH; [| apply Hcan_link]. congruence. }
   { exfalso. match goal with H:_|-_ => apply mk_is_Some in H; apply fill_val in H; destruct H as [? HH] end.
     rewrite /to_val to_of_class // in HH. }
-  rename H0 into Hfill. rename H4 into Hnofn. rewrite proj1_prog_union in Hnofn;[|apply Hcan_link].
+  rename H into Hfill. rename H3 into Hnofn. rewrite proj1_prog_union in Hnofn;[|apply Hcan_link].
   pose proof (call_in_ctx_to_val _ _ _ _ _ Hfill) as [[K'' ->]|Hval].
   2: { exfalso. unfold to_val in Hval. destruct Hval. by repeat case_match. }
   rewrite -fill_comp in Hfill. apply fill_inj in Hfill. subst e1.
@@ -384,12 +310,12 @@ Proof using.
   destruct HH as [->|[? HH]].
   2: { exfalso. rewrite to_of_class in HH. congruence. }
   do 3 eexists; repeat split; eauto.
-  rewrite fill_empty to_of_class in H3. by simplify_eq/=.
+  rewrite fill_empty to_of_class in H2. by simplify_eq/=.
 Qed.
 
-Lemma link_head_step_call_ext_2_inv INVG pe1 pe2 K f vs σ2 privσ1 X :
-  let pe := link_environ INVG pe1 pe2 in
-  can_link_prog INVG pe1 pe2 →
+Lemma link_head_step_call_ext_2_inv `{!invGS_gen hlc Σ} pe1 pe2 K f vs σ2 privσ1 X :
+  let pe := link_environ pe1 pe2 in
+  can_link_prog pe1 pe2 →
   prog pe2 !! f = None →
   head_step (prog pe) (LkSE (LinkExpr2 Λ1 Λ2 (fill K (of_class Λ2 (ExprCall f vs)))),
                        LinkSt2 privσ1 σ2) X →
@@ -403,7 +329,7 @@ Proof using.
     rewrite proj2_prog_union in HH; [| apply Hcan_link]. congruence. }
   { exfalso. match goal with H:_|-_ => apply mk_is_Some in H; apply fill_val in H; destruct H as [? HH] end.
     rewrite /to_val to_of_class // in HH. }
-  rename H0 into Hfill. rename H4 into Hnofn. rewrite proj2_prog_union in Hnofn;[|apply Hcan_link].
+  rename H into Hfill. rename H3 into Hnofn. rewrite proj2_prog_union in Hnofn;[|apply Hcan_link].
   pose proof (call_in_ctx_to_val _ _ _ _ _ Hfill) as [[K'' ->]|Hval].
   2: { exfalso. unfold to_val in Hval. destruct Hval. by repeat case_match. }
   rewrite -fill_comp in Hfill. apply fill_inj in Hfill. subst e2.
@@ -411,16 +337,16 @@ Proof using.
   destruct HH as [->|[? HH]].
   2: { exfalso. rewrite to_of_class in HH. congruence. }
   do 3 eexists; repeat split; eauto.
-  rewrite fill_empty to_of_class in H3. by simplify_eq/=.
+  rewrite fill_empty to_of_class in H2. by simplify_eq/=.
 Qed.
 
-Lemma wp_link_run (INVG: invGS_gen hlc Σ)
-  (pe1 : @prog_environ hlc _ _ Λ1 Σ (IrisG INVG state_interp1))
-  (pe2 : @prog_environ hlc _ _ Λ2 Σ (IrisG INVG state_interp2))
+Lemma wp_link_run `{!invGS_gen hlc Σ}
+  (pe1 : @prog_environ _ _ _ _ _ _ Λ1 _)
+  (pe2 : @prog_environ _ _ _ _ _ _ Λ2 _)
   E
 :
-  let pe := link_environ INVG pe1 pe2 in
-  can_link_prog INVG pe1 pe2 →
+  let pe := link_environ pe1 pe2 in
+  can_link_prog pe1 pe2 →
   ⊢ □ (
     (∀ e1 Φ, WP e1 @ pe1; E {{ Φ }} -∗
              WP (LkSE (LinkExpr1 Λ1 Λ2 e1)) @ pe; E {{ Φ }}) ∗
@@ -432,9 +358,9 @@ Proof using.
   (* Case 1: running Λ1 *)
   { iIntros (e1 Φ) "Hwp".
     rewrite wp_unfold. rewrite /wp_pre.
-    iApply (@wp_unfold _ _ _ (link_lang Λ1 Λ2)). rewrite /wp_pre.
+    iApply (@wp_unfold _ _ _ _ _ _ (link_lang Λ1 Λ2)). rewrite /wp_pre.
     iIntros (σ) "[Hσ %Hmatch]".
-    inversion Hmatch; subst. iDestruct "Hσ" as "(Hσ1 & Hpriv2 & %Hvsplit)".
+    inversion Hmatch; subst. iDestruct "Hσ" as "(Hσ1 & Hpriv2)".
     iMod ("Hwp" $! σ1 with "[$Hσ1]") as "[Hwp|[Hwp|Hwp]]"; first done.
 
     (* WP: value case *)
@@ -447,24 +373,20 @@ Proof using.
       iIntros (X Hstep). apply head_reducible_prim_step in Hstep; [|done].
       inversion Hstep; simplify_eq/=.
       { exfalso. by match goal with H:_ |- _ => apply val_prim_step in H end. }
-      { rewrite /to_val to_of_class in H4; simplify_eq/=.
-        iMod (@state_interp_split _ _ _ public_state_interp Λ1 with "Hσ") as "[Hpriv1 Hpub]"; first by eauto.
+      { rewrite /to_val to_of_class in H3; simplify_eq/=.
+        iMod (@state_interp_split _ _ _ _ Λ1 with "Hσ") as "[Hpriv1 Hpub]"; first by eauto.
         iExists _, _. iSplitR; first done. iFrame. do 3 iModIntro.
-        iSplitR.
-        { iPureIntro. split; first by (eexists; eauto).
-          destruct Hvsplit as (σ1_0 & pubσ0 & privσ1_0 & Hrel0 & Hsplit0 & Hvsplit).
-          eapply (lang1_state_rel_valid_split σ1_0); eauto. }
         by iApply wp_value. }
       { exfalso.
         assert (is_Some (to_val e1)) as [? ?].
-        { eapply fill_val. eexists. unfold to_val. erewrite H0. rewrite to_of_class//. }
-        unfold to_val in H1. repeat case_match; congruence. } }
+        { eapply fill_val. eexists. unfold to_val. erewrite H. rewrite to_of_class//. }
+        unfold to_val in H0. repeat case_match; congruence. } }
 
     (* WP: call case *)
     { iDestruct "Hwp" as (f vs K -> Hf) "Hcall". iModIntro. iRight; iRight.
       (* administrative step MakeCall1S: LinkExpr1 ~> LinkExprCall *)
       assert (head_reducible (prog pe) (LkSE (LinkExpr1 Λ1 Λ2 (fill K (of_class Λ1 (ExprCall f vs))))) (LinkSt1 σ1 privσ2)).
-      { apply matching_expr_state_ctx in H3.
+      { apply matching_expr_state_ctx in H2.
         destruct (call_matching_split _ _ _ ltac:(eassumption)) as (?&?&?).
         exists (λ _, True). eapply MakeCall1S; eauto. by rewrite to_of_class.
         rewrite proj1_prog_union; [done | apply Hcan_link]. }
@@ -473,11 +395,8 @@ Proof using.
       eapply link_head_step_call_ext_1_inv in Hstep as (pubσ&privσ1&k1&->&?&?); eauto.
 
       iMod "Hcall" as "[Hσ Hcall]". iDestruct "Hcall" as (Ξ) "[HTΞ HΞ]".
-      iMod (@state_interp_split _ _ _ public_state_interp Λ1 with "Hσ") as "[Hpriv1 Hpub]"; eauto.
-      iModIntro. iNext. iModIntro. iExists _, _. iSplitR; first done. iFrame. iSplitR.
-      { iPureIntro. split; first by (eexists; eauto).
-        destruct Hvsplit as (σ1_0 & pubσ0 & privσ1_0 & Hrel0 & Hsplit0 & Hvsplit).
-        eapply (lang1_state_rel_valid_split σ1_0); eauto. }
+      iMod (@state_interp_split _ _ _ _ Λ1 with "Hσ") as "[Hpriv1 Hpub]"; eauto.
+      iModIntro. iNext. iModIntro. iExists _, _. iSplitR; first done. iFrame.
 
       (* two cases: this is an external call of the linking module itself, or it
          is a call to a function of pe2 *)
@@ -494,8 +413,8 @@ Proof using.
 
         progress change (LkE (LinkExpr2 Λ1 Λ2 e2) [inl k1]) with
           (linking.fill _ _ ([inl k1]:ectx (link_lang Λ1 Λ2)) (LkSE (LinkExpr2 Λ1 Λ2 e2))).
-        iApply (@wp_bind _ _ _ (link_lang Λ1 Λ2)).
-        iApply ((@wp_wand _ _ _ (link_lang Λ1 Λ2)) with "[Hwpcall]").
+        iApply (@wp_bind _ _ _ _ _ _ (link_lang Λ1 Λ2)).
+        iApply ((@wp_wand _ _ _ _ _ _ (link_lang Λ1 Λ2)) with "[Hwpcall]").
         { iDestruct "IH" as "#[_ IH2]". iApply "IH2". iApply "Hwpcall". }
         iIntros (r) "Hr". iSpecialize ("HΞ" with "Hr"). rewrite -fill_comp fill_empty. simpl.
 
@@ -521,25 +440,22 @@ Proof using.
       iIntros (X Hstep). apply head_reducible_prim_step in Hstep;[|done].
       inversion Hstep; simplify_eq.
       { (* non-vacuous case: step in Λ1 *)
-        clear Hstep. rename H6 into Hstep. apply lang1_state_rel_prim_step in Hstep.
+        clear Hstep. rename H5 into Hstep.
         rewrite proj1_prog_union in Hstep; [|apply Hcan_link].
-        iSpecialize ("Hwp" $! _ Hstep). iMod "Hwp". iIntros "!>!>". iMod "Hwp" as (e' σ' [HX HrX]) "[Hσ Hwp]".
-        iModIntro. iExists _, _. iSplitR; [iPureIntro; naive_solver|].
-        iSplitL "Hσ Hpriv2".
-        { simpl. iFrame. iPureIntro. destruct Hvsplit as (σ1_0 & pubσ0 & privσ1_0 & Hrel0 & Hsplit0 & Hvsplit).
-          eexists σ1_0, pubσ0, _. repeat split; eauto. etransitivity; eauto. }
+        iSpecialize ("Hwp" $! _ Hstep). iMod "Hwp". iIntros "!>!>". iMod "Hwp" as (e' σ' HX) "[Hσ Hwp]".
+        iModIntro. iExists _, _. iSplitR; [iPureIntro; naive_solver|]. iFrame.
         iDestruct "IH" as "[IH1 _]". iApply ("IH1" with "Hwp"). }
       { exfalso. apply reducible_not_val in Hred. congruence. }
       { exfalso. clear Hstep. erewrite <-(of_to_class e0) in Hred; [|eassumption].
-        rewrite proj1_prog_union in H6;[|apply Hcan_link].
+        rewrite proj1_prog_union in H5;[|apply Hcan_link].
         destruct Hred as (?&Hred). eapply extcall_ctx_irreducible; eauto. } } }
 
   (* Case 2: running Λ2 *)
   { iIntros (e2 Φ) "Hwp".
     rewrite wp_unfold. rewrite /wp_pre.
-    iApply (@wp_unfold _ _ _ (link_lang Λ1 Λ2)). rewrite /wp_pre.
+    iApply (@wp_unfold _ _ _ _ _ _ (link_lang Λ1 Λ2)). rewrite /wp_pre.
     iIntros (σ) "[Hσ %Hmatch]".
-    inversion Hmatch; subst. iDestruct "Hσ" as "(Hprivσ1 & Hσ2 & %Hvsplit)".
+    inversion Hmatch; subst. iDestruct "Hσ" as "(Hprivσ1 & Hσ2)".
     iMod ("Hwp" $! σ2 with "[$Hσ2]") as "[Hwp|[Hwp|Hwp]]"; first done.
 
     (* WP: value case *)
@@ -552,24 +468,20 @@ Proof using.
       iIntros (X Hstep). apply head_reducible_prim_step in Hstep; [|done].
       inversion Hstep; simplify_eq/=.
       { exfalso. by match goal with H:_ |- _ => apply val_prim_step in H end. }
-      { rewrite /to_val to_of_class in H4; simplify_eq/=.
-        iMod (@state_interp_split _ _ _ public_state_interp Λ2 with "Hσ") as "[Hpriv2 Hpub]"; first by eauto.
+      { rewrite /to_val to_of_class in H3; simplify_eq/=.
+        iMod (@state_interp_split _ _ _ _ Λ2 with "Hσ") as "[Hpriv2 Hpub]"; first by eauto.
         iExists _, _. iSplitR; first done. iFrame. iModIntro. iNext. iModIntro.
-        iSplitR.
-        { iPureIntro. split; last by (eexists; eauto).
-          destruct Hvsplit as (σ2_0 & pubσ0 & privσ2_0 & Hrel0 & Hsplit0 & Hvsplit).
-          eapply (lang2_state_rel_valid_split σ2_0); eauto. }
         by iApply wp_value. }
       { exfalso.
         assert (is_Some (to_val e2)) as [? ?].
-        { eapply fill_val. eexists. unfold to_val. erewrite H0. rewrite to_of_class//. }
-        unfold to_val in H1. repeat case_match; congruence. } }
+        { eapply fill_val. eexists. unfold to_val. erewrite H. rewrite to_of_class//. }
+        unfold to_val in H0. repeat case_match; congruence. } }
 
     (* WP: call case *)
     { iDestruct "Hwp" as (f vs K -> Hf) "Hcall". iModIntro. iRight; iRight.
       (* administrative step MakeCall1S: LinkExpr2 ~> LinkExprCall *)
       assert (head_reducible (prog pe) (LkSE (LinkExpr2 Λ1 Λ2 (fill K (of_class Λ2 (ExprCall f vs))))) (LinkSt2 privσ1 σ2)).
-      { apply matching_expr_state_ctx in H3.
+      { apply matching_expr_state_ctx in H2.
         destruct (call_matching_split _ _ _ ltac:(eassumption)) as (?&?&?).
         exists (λ _, True). eapply MakeCall2S; eauto. by rewrite to_of_class.
         rewrite proj2_prog_union; [done | apply Hcan_link]. }
@@ -578,11 +490,8 @@ Proof using.
       eapply link_head_step_call_ext_2_inv in Hstep as (pubσ&privσ2&k2&->&?&?); eauto.
 
       iMod "Hcall" as "[Hσ Hcall]". iDestruct "Hcall" as (Ξ) "[HTΞ HΞ]".
-      iMod (@state_interp_split _ _ _ public_state_interp Λ2 with "Hσ") as "[Hpub Hpriv2]"; eauto.
-      iModIntro. iNext. iModIntro. iExists _, _. iSplitR; first done. iFrame. iSplitR.
-      { iPureIntro. split; last by (eexists; eauto).
-        destruct Hvsplit as (σ2_0 & pubσ0 & privσ2_0 & Hrel0 & Hsplit0 & Hvsplit).
-        eapply (lang2_state_rel_valid_split σ2_0); eauto. }
+      iMod (@state_interp_split _ _ _ _ Λ2 with "Hσ") as "[Hpub Hpriv2]"; eauto.
+      iModIntro. iNext. iModIntro. iExists _, _. iSplitR; first done. iFrame.
 
       (* two cases: this is an external call of the linking module itself, or it
          is a call to a function of pe2 *)
@@ -599,8 +508,8 @@ Proof using.
 
         progress change (LkE (LinkExpr1 Λ1 Λ2 e1) [inr k2]) with
           (linking.fill _ _ ([inr k2]:ectx (link_lang Λ1 Λ2)) (LkSE (LinkExpr1 Λ1 Λ2 e1))).
-        iApply (@wp_bind _ _ _ (link_lang Λ1 Λ2)).
-        iApply ((@wp_wand _ _ _ (link_lang Λ1 Λ2)) with "[Hwpcall]").
+        iApply (@wp_bind _ _ _ _ _ _ (link_lang Λ1 Λ2)).
+        iApply ((@wp_wand _ _ _ _ _ _ (link_lang Λ1 Λ2)) with "[Hwpcall]").
         { iDestruct "IH" as "#[IH1 _]". iApply "IH1". iApply "Hwpcall". }
         iIntros (r) "Hr". iSpecialize ("HΞ" with "Hr"). rewrite -fill_comp fill_empty. simpl.
 
@@ -627,16 +536,14 @@ Proof using.
       iIntros (X Hstep). apply head_reducible_prim_step in Hstep;[|done].
       inversion Hstep; simplify_eq.
       { (* non-vacuous case: step in Λ2 *)
-        clear Hstep. rename H6 into Hstep. apply lang2_state_rel_prim_step in Hstep.
+        clear Hstep. rename H5 into Hstep.
         rewrite proj2_prog_union in Hstep; [|apply Hcan_link].
-        iSpecialize ("Hwp" $! _ Hstep). iMod "Hwp". iIntros "!>!>". iMod "Hwp" as (e' σ' [HX HrX]) "[Hσ Hwp]".
-        iModIntro. iExists _, _. iSplitR; [iPureIntro; naive_solver|]. iSplitL "Hσ Hprivσ1".
-        { simpl. iFrame. iPureIntro. destruct Hvsplit as (σ2_0 & pubσ0 & privσ2_0 & Hrel0 & Hsplit0 & Hvsplit).
-          eexists σ2_0, pubσ0, _. repeat split; eauto. etransitivity; eauto. }
+        iSpecialize ("Hwp" $! _ Hstep). iMod "Hwp". iIntros "!>!>". iMod "Hwp" as (e' σ' HX) "[Hσ Hwp]".
+        iModIntro. iExists _, _. iSplitR; [iPureIntro; naive_solver|]. iFrame.
         iDestruct "IH" as "[_ IH2]". iApply ("IH2" with "Hwp"). }
       { exfalso. apply reducible_not_val in Hred. congruence. }
       { exfalso. clear Hstep. erewrite <-(of_to_class e0) in Hred; [|eassumption].
-        rewrite proj2_prog_union in H6;[|apply Hcan_link].
+        rewrite proj2_prog_union in H5;[|apply Hcan_link].
         destruct Hred as (?&Hred). eapply extcall_ctx_irreducible; eauto. } } }
 Qed.
 
